type_sys: refactor for branch left,right,both paths

theories/Impl.v
@@ -11,6 +11,20 @@ From RocqCandy Require Import All.
 From CoplandSpec Require Import Term_Defs.
 From CVM Require Import Monad.
 
+Definition proc_ev_path_left_ev (ep : ev_path) e : Evidence :=
+  match ep with
+  | left_path => e
+  | right_path => mt_evc
+  | both_paths => e
+  end.
+
+Definition proc_ev_path_right_ev (ep : ev_path) e : Evidence :=
+  match ep with
+  | left_path => mt_evc
+  | right_path => e
+  | both_paths => e
+  end.
+
 (** Monadic CVM implementation (top-level) *)
 Fixpoint build_cvm (e : Evidence) (t: Term) : CVM Evidence :=
   match t with
@@ -20,18 +34,18 @@ Fixpoint build_cvm (e : Evidence) (t: Term) : CVM Evidence :=
     e1 <- build_cvm e t1 ;;cvm
     build_cvm e1 t2
 
-  | bseq t1 t2 =>
+  | bseq ep t1 t2 =>
     split_ev ;;cvm
-    e1r <- build_cvm e t1 ;;cvm
-    e2r <- build_cvm e t2 ;;cvm
+    e1r <- build_cvm (proc_ev_path_left_ev ep e) t1 ;;cvm
+    e2r <- build_cvm (proc_ev_path_right_ev ep e) t2 ;;cvm
     join_seq e1r e2r
 
-  | bpar t1 t2 =>
+  | bpar ep t1 t2 =>
     split_ev ;;cvm
     (* We will make the LOC = event_id for start of thread *)
     (* start a parallel thread working on the evidence split for t2 *)
     loc <- start_par_thread e t2 ;;cvm
-    e1r <- build_cvm e t1 ;;cvm
-    e2r <- wait_par_thread loc e t2 ;;cvm
+    e1r <- build_cvm (proc_ev_path_left_ev ep e) t1 ;;cvm
+    e2r <- wait_par_thread loc (proc_ev_path_right_ev ep e) t2 ;;cvm
     join_seq e1r e2r
   end.
